So much planning and fixing and pushing to the future, gahhhhhhh! But I have a cafe to cheer me up :))

Proof/Algorithm/Cycle.lean
@@ -6,16 +6,46 @@ open Proof (Program)
 
 -- by the less than all fixpoints lemma, since algoRE has G G₀ (from .cycle),
 -- So does all fixpoints.
+-- ie. RE G G₀
 -- prove h : for any config, G _ _ S _, forall G' in S, G ∈ Dep G' (induction over steps)
--- have hdep : G' ∈ Dep G by definition
+-- have hdep : G' ∈ Dep G by definition of RE
 -- Now by .cycle either G₀ = G or G₀ on stack
 -- if first, exact hdep
 -- else, by h, we have trans cycle
 
+def StackDep (L : Program) : Config → Prop
+  | .mk G _ F S _ =>
+      ∀ G' ∈ S.globs, G ∈ Proof.Dep F.glue L G'
+  | .cycle _ => True
+  | .done _ => True
+
+-- I don't like the above. Should just make a Dep for Algo...
+-- Then prove that G is in AlgoDep G'.
+-- Prove that AlgoRE is always less than RE. And so AlgoDep is always
+-- less than Dep in LessThanInv.
+-- then we have the fact that ∀ σ : Proof.Sigma, Proof.FixPoint σ L → G ∈ Proof.Dep σ L G'
+
+theorem stack_dep_step {c c' : Config} {L : Program} {hL : L.HasMain}
+    (hstep : Solve L c c') (h : StackDep L c) :
+    StackDep L c' := sorry
+
+theorem stack_dep_star {c : Config} {L : Program} {hL : L.HasMain}
+    (hstar : Solve.Star L (Config.start L hL) c) :
+    StackDep L c := sorry
 
 theorem report_cycle_then_dep {L : Program} {hL : L.HasMain} :
-    ∃ G, Solve.Star L (Config.start L hL) (.cycle G) →
+    ∀ G, Solve.Star L (Config.start L hL) (.cycle G) →
     ∀ σ : Proof.Sigma, Proof.FixPoint σ L → G ∈ Proof.Dep σ L G := by
-  sorry
+  intro G hcyc σ hf
+  obtain _ | ⟨h_star, h_step⟩ := hcyc
+  rename_i c_prev
+  rcases c_prev with ⟨ G', σ', F, S, Q ⟩ | F | G'
+  · cases h_step with
+    | cycle hare hneeds hG =>
+      -- have hre : Proof.RE σ L G := by LessThanInv hare combined with F is less than σ
+
+    sorry
+  · cases h_step
+  · cases h_step
 
 end Algorithm
